src/FcEtt/ett_match.v
@@ -1,0 +1,20 @@
+Set Bullet Behavior "Strict Subproofs".
+Set Implicit Arguments.
+
+Require Export FcEtt.tactics.
+Require Export FcEtt.imports.
+Require Import FcEtt.utils.
+
+Require Export FcEtt.ett_inf.
+Require Export FcEtt.ett_ott.
+Require Export FcEtt.ett_ind.
+
+Lemma match_subst_lc : forall a p b b', MatchSubst a p b b' -> lc_tm a ->
+                                        lc_tm b -> lc_tm b'.
+Proof. intros. induction H.
+        - auto.
+        - inversion H0; subst. apply tm_subst_tm_tm_lc_tm; auto.
+        - inversion H0; subst. apply tm_subst_tm_tm_lc_tm; auto.
+        - inversion H0; subst. apply tm_subst_tm_tm_lc_tm; auto.
+        - inversion H0; subst. apply co_subst_co_tm_lc_tm; auto.
+Qed.
